src/Iris/Algebra/Lib/ClassicalHeaps.lean
@@ -8,6 +8,72 @@ import Iris.Algebra.Heap
 
 -- Library functions: move me
 
+/-- A set whose complement is infinite -/
+def coinfinite (S : P → Prop) : Prop :=
+  ∃ f : Nat → P, (∀ n, S <| f n) ∧ (∀ n m : Nat, f n = f m → n = m)
+
+/-- Arbitrarily changing one element of a co-infinite set yields a co-infinite set -/
+theorem cofinite_alter_cofinite {S S' : P → Prop} (p' : P) (Ha : ∀ p, p ≠ p' → S p = S' p)
+    (Hs : coinfinite S) : coinfinite S' := by
+  rcases Hs with ⟨f, HfS, Hfinj⟩
+  -- Basically, alter f so that f never hits p'.
+  rcases (Classical.em (∃ n, f n = p')) with (⟨n, H⟩|H)
+  · exists fun n' => if n' < n then f n' else f n'.succ
+    constructor
+    · intro n'
+      simp only []
+      split
+      · rw [← Ha]
+        · apply HfS
+        · rename_i Hk'
+          intro Hk
+          exact Nat.lt_irrefl (n := n) <| (Hfinj _ _ (Hk ▸ H)) ▸ Hk'
+      · rw [← Ha]
+        · apply HfS
+        · rename_i Hk'
+          intro Hk
+          have _ := (Hfinj _ _ (Hk ▸ H)) ▸ Hk'
+          simp_all
+    · intro n' m'
+      simp only []
+      split <;> split
+      · apply Hfinj
+      · intro H
+        have Hfinj' := Hfinj _ _ H
+        exfalso
+        subst Hfinj'
+        rename_i HK HK'
+        apply HK
+        exact Nat.lt_of_succ_lt HK'
+      · intro H
+        have Hfinj' := Hfinj _ _ H
+        exfalso
+        subst Hfinj'
+        rename_i HK HK'
+        apply HK
+        exact Nat.lt_of_succ_lt HK'
+      · intro H
+        exact Nat.succ_inj.mp (Hfinj n'.succ m'.succ H)
+  · exists f
+    refine ⟨?_, Hfinj⟩
+    exact fun n => (Ha _ (H ⟨n, ·⟩)) ▸ HfS n
+
+open Classical in
+/- Update a (classical) function at a point. Used to specify the correctness of stores. -/
+noncomputable def fset {K V : Type _} (f : K → V) (k : K) (v : V) : K → V :=
+  fun k' => if (k = k') then v else f k'
+
+@[simp] def support (f : K → Option V) : K → Prop := ((· == true) ∘ Option.isSome ∘ f)
+
+theorem coinfinite_fset_coinfinite (f : K → Option V) (H : coinfinite (support f)) :
+    coinfinite (support (fset f k v)) := by
+  apply cofinite_alter_cofinite  k _ H
+  intro p Hpk
+  simp [support, fset]
+  split
+  · simp_all
+  · rfl
+
 
 -- TODO: Move do a library file?
 section instances
@@ -15,10 +81,10 @@ section instances
 noncomputable def instClassicalStore {K V : Type _} : Store (K → V) K V where
   get := id
   set := fset
-  of_fun := id
+  ofFun := id
   get_set_eq H := by rw [H]; simp [fset]
   get_set_ne H := by simp_all [fset]
-  of_fun_get := rfl
+  ofFun_get := rfl
 
 noncomputable def instClassicalHeap : Heap (K → Option V) K V where
   toStore := instClassicalStore
@@ -37,8 +103,10 @@ for example, express an infinite number of pices of ghost state while retaining 
 allocate new ghost state. -/
 noncomputable def instClassicaAllocHeap : AllocHeap (K → Option V) K V where
   toHeap := instClassicalHeap
-  fresh HC _ := Classical.choose (coinfinte_exists_next HC)
-  fresh_get HC := Classical.choose_spec (coinfinte_exists_next HC)
+  notFull f := coinfinite <| support f
+  fresh HC := Classical.choose (coinfinte_exists_next HC)
+  fresh_get {_ HC} := Classical.choose_spec (coinfinte_exists_next HC)
+  notFull_set_fresh {_ H _} := coinfinite_fset_coinfinite _ H
 
 -- TODO: Heaps indexed by natural numbers. Still a generalization over Iris because
 -- an infinite number of values can be givien non-default values!
